lib/coq/todo.md
@@ -1,20 +1,28 @@
 # For testing purpose
 
 ## Inputing
-- Port and adapt Guillaume's surface syntaxe in Coq for CFML
-- Write down Fibonacci
+- [DONE] Port and adapt Guillaume's surface syntaxe in Coq for CFML
+- [Somewhat DONE] Write down Fibonacci
 
 ## Computing
-- problem with computability of maps -> move to CompCert's PTrees
-- PTrees: no union operation defined? To add?
-- Need to convert cfml's vars to AST.ident == positive to this end
+- [DONE] problem with computability of maps -> move to CompCert's PTrees
+- [DONE] PTrees: no union operation defined? To add?
+- [DONE: added `option ident` to the `var` type] Need to convert
+  cfml's vars to AST.ident == positive to this end
 
 # On ident generation
 - Reusing essentially the [mon] monad from CompCert that is more or less [FreshT fail]
-- Question of initial seed: should be fine to just use 0 for us
-- Question of tracking ident to source name: duplicate locally [mon] with an extended [trail] field?
+- Question of initial seed: should be fine to just use ~~0~~ 1
+  (`positive` > 0) for us
+- Question of tracking ident to source name: duplicate locally [mon]
+  with an extended [trail] field?
 
 # Semantics
 
-- omnismall for clight statements
-- remove subst for cfml omnismall, and add envs
+- omnismall for clight statements -> [Workaround: defined *eventually*
+  judgement from Clight's small step]
+- [DONE] remove subst for cfml omnismall, and add envs
+- Rewrite memory model of CFML_C to be closer to Clight's
+  (*ie* `block -> offset -> val`)
+- Maybe Add traces to CFML_C's semantic?
+- Actually refactor semantics (cf Clight.state)
